case_studies/HamiltonBlum/Blum_ZK.ec
@@ -1,6 +1,5 @@
 pragma Goals:printall.
 require import AllCore DBool Bool List Distr Int Aux DJoin.
-
 require import Permutation Blum_Basics Blum_Sim1Property.
 
 import DJMM.
@@ -10,8 +9,6 @@ clone import Statistical with op epsilon <- 2%r * negl + 20%r * negl2,
                               op sigma <- (1%r/2%r - negl2).
 
 
-
-(* clone import StatisticalZKDeriv with op negl <- 2%r * negl + 20%r * negl2. *)
 axiom negl2_prop : 0%r <= negl2 < 1%r/4%r.
 
 require RewBasics.
@@ -44,7 +41,7 @@ declare axiom rewindable_V_plus :
 
 
 lemma hc_statistical_zk stat wit  &m:
-        IsHC (stat, wit) => 
+        zk_relation stat wit => 
         let real_prob = Pr[ZKReal(HonestProver, V, D).run(stat, wit) @ &m : res] in
         let ideal_prob = Pr[ZKIdeal(SimN(Sim1), V, D).run(stat, wit) @ &m : res] in
           `|ideal_prob - real_prob| <= (2%r * negl + 20%r * negl2) + 2%r * (1%r- (1%r/2%r - negl2)) ^ OSS.N.
@@ -54,17 +51,15 @@ apply (statistical_zk HonestProver Sim1  V D _ _ _ _ _ _ _ _ _ _  stat wit &m _)
 apply D_guess_ll. 
 proc*. call D_guess_prop. skip.  auto.
 move => x.
-
-(* apply (sim1_rew_ph V _ _ _ x). *) admit. (* apply V_summitup_ll. apply V_challenge_ll. *)
-(* apply (rewindable_A_plus V). apply rewindable_V_plus. *)
-
-
+apply (sim1_rew_ph V _ _ _ _ _ x). apply V_summitup_ll. apply V_challenge_ll. apply P_response_ll. apply P_commitment_ll.
+apply (rewindable_A_plus V). apply rewindable_V_plus.
 progress.
-apply (sim1_prop V D  _ _  _ _ _  &m0 p w  _ );auto.  apply (rewindable_A_plus V). apply rewindable_V_plus. 
+apply (sim1_prop V D  _ _  _ _ _  _ &m0 p w  _ );auto.  apply V_summitup_ll. apply (rewindable_A_plus V). apply rewindable_V_plus. 
 apply D_guess_ll. apply V_summitup_ll. apply V_challenge_ll. smt (negl2_prop).
 progress.
-apply (sim1assc V D _ _ _ _ _ &m0 stat0 _).  apply (rewindable_A_plus V). apply rewindable_V_plus. apply D_guess_ll. apply V_summitup_ll.
-apply V_challenge_ll. apply negl2_prop. admit.
+apply (sim1assc V D _ _ _ _ _ _ &m0 stat0 _).  apply V_summitup_ll. apply (rewindable_A_plus V). apply rewindable_V_plus. apply D_guess_ll. apply V_summitup_ll.
+apply V_challenge_ll. apply negl2_prop. 
+elim H0. progress. smt.
 auto.
 qed.
 
